Merge StructLiteral.fsti with fst for now

examples/steel/arraystructs/Steel.C.StructLiteral.fst
@@ -13,10 +13,85 @@ open Steel.C.Connection
 open FStar.List.Tot
 open FStar.FunctionalExtensionality
 
+(**** BEGIN PUBLIC *)
+
+let struct_fields =
+  struct_fields:list (string * typedef){Cons? struct_fields}
+
+[@@__reduce__]
+let rec mem (#a:eqtype) (x:a) (xs:list a)
+: Pure bool (requires True) (ensures fun b -> b == List.Tot.mem x xs)
+= match xs with
+  | [] -> false
+  | x' :: xs -> x = x' || x `mem` xs
+
+[@@__reduce__]
+let rec map (f: 'a -> 'b) (xs:list 'a)
+: Pure (list 'b) (requires True) (ensures fun b -> b == List.Tot.map f xs)
+= match xs with
+  | [] -> []
+  | x :: xs -> f x :: map f xs
+
+[@@__reduce__]
+let has_field_bool (fields: struct_fields) (field: string): bool =
+  field `mem` map fst fields
+
+[@@iter_unfold]
+let has_field (fields: struct_fields) (field: string): prop =
+  has_field_bool fields field == true
+
+let field_of (fields: struct_fields) =
+  refine string (has_field fields)
+
+[@@__reduce__;iter_unfold]
+let mk_field_of (fields: struct_fields) (field: string)
+: Pure (field_of fields)
+    (requires normalize_term (has_field_bool fields field) == true)
+    (ensures fun field' -> field' == field)
+= field
+
+[@@__reduce__]
+let rec get_field (fields: struct_fields) (field: field_of fields): typedef =
+  match fields with
+  | (field', td) :: fields -> if field = field' then td else get_field fields field
+
+/// A view type for structs
+
+[@@__reduce__]
+let struct_views (fields: struct_fields) (field: field_of fields)
+: sel_view ((get_field fields field).pcm) ((get_field fields field).view_type) false
+= (get_field fields field).view
+
 let struct_view_types (fields: struct_fields) (field: field_of fields) =
   (get_field fields field).view_type
 
+val struct (tag: string) (fields: struct_fields): Type0
+(**** END PUBLIC *)
+
 let struct tag fields = restricted_t (field_of fields) (struct_view_types fields)
+
+(**** BEGIN PUBLIC *)
+let rec list_fn (dom: list Type) (cod: Type) = match dom with
+  | [] -> cod
+  | d :: dom -> d -> list_fn dom cod
+
+let rec list_fn_map #dom (f: 'a -> 'b) (g: dom `list_fn` 'a): dom `list_fn` 'b = match dom with 
+  | [] -> f g <: [] `list_fn` 'b
+  | d :: dom' ->
+    let g: d -> dom' `list_fn` 'a = g in
+    fun (x:d) -> list_fn_map f (g x) <: dom' `list_fn` 'b
+
+let struct_field_view_type ((_, td): string * typedef): Type = td.view_type
+
+let mk_struct_ty_dom (tag: string) (fields: list (string * typedef)): list Type =
+  map struct_field_view_type fields
+
+let mk_struct_ty (tag: string) (fields: struct_fields): Type =
+  mk_struct_ty_dom tag fields `list_fn` struct tag fields
+
+/// A struct literal
+val mk_struct (tag: string) (fields: struct_fields): mk_struct_ty tag fields
+(**** END PUBLIC *)
 
 let rec mk_struct (tag: string) (fields: struct_fields)
 : mk_struct_ty tag fields
@@ -31,6 +106,73 @@ let rec mk_struct (tag: string) (fields: struct_fields)
       in on_dom _ h
     in
     list_fn_map lift_struct f
+
+(**** BEGIN PUBLIC *)
+/// Reading a struct field
+val struct_get
+  (#tag: string) (#fields: struct_fields)
+  (x: struct tag fields) (field: field_of fields)
+: (get_field fields field).view_type
+
+/// Writing a struct field
+val struct_put
+  (#tag: string) (#fields: struct_fields)
+  (x: struct tag fields)
+  (field: field_of fields)
+  (v: (get_field fields field).view_type)
+: struct tag fields
+
+/// For a fixed field name, struct_get and struct_put form a lens
+
+val struct_get_put 
+  (#tag: string) (#fields: struct_fields)
+  (x: struct tag fields)
+  (field: field_of fields)
+  (v: (get_field fields field).view_type)
+: Lemma (struct_put x field v `struct_get` field == v)
+  [SMTPat (struct_put x field v `struct_get` field)]
+
+val struct_put_get
+  (#tag: string) (#fields: struct_fields)
+  (x: struct tag fields)
+  (field: field_of fields)
+: Lemma (struct_put x field (x `struct_get` field) == x)
+  [SMTPat (struct_put x field (x `struct_get` field))]
+
+val struct_put_put
+  (#tag: string) (#fields: struct_fields)
+  (x: struct tag fields)
+  (field: field_of fields)
+  (v w: (get_field fields field).view_type)
+: Lemma (struct_put (struct_put x field v) field w == struct_put x field w)
+  [SMTPat (struct_put (struct_put x field v) field w)]
+
+/// struct_get/struct_put pairs for different fields don't interfere with each other
+
+val struct_get_put_ne
+  (#tag: string) (#fields: struct_fields)
+  (x: struct tag fields)
+  (field1: field_of fields)
+  (field2: field_of fields)
+  (v: (get_field fields field1).view_type)
+: Lemma
+    (requires field1 =!= field2)
+    (ensures struct_put x field1 v `struct_get` field2 == x `struct_get` field2)
+  [SMTPat (struct_put x field1 v `struct_get` field2)]
+  
+val struct_put_put_ne
+  (#tag: string) (#fields: struct_fields)
+  (x: struct tag fields)
+  (field1: field_of fields)
+  (v: (get_field fields field1).view_type)
+  (field2: field_of fields)
+  (w: (get_field fields field2).view_type)
+: Lemma
+    (requires field1 =!= field2)
+    (ensures
+      struct_put (struct_put x field1 v) field2 w ==
+      struct_put (struct_put x field2 w) field1 v)
+(**** END PUBLIC *)
 
 let struct_get x field = x field
 
@@ -51,141 +193,38 @@ let struct_put_put_ne x field1 v field2 w =
     struct_put (struct_put x field1 v) field2 w `feq`
     struct_put (struct_put x field2 w) field1 v)
 
-(*
-define attribute on mk_struct_view_type, etc..
+(**** BEGIN PUBLIC *)
+/// Similarly, a PCM for structs
 
-mk_struct_view': fields:list (string * _) ->
-  norm [delta_attr ..; delta Fstar.list.map; ..] .. (mk_struct_view_type fields ..)
-  (See FStar.Pervasives.fsti)
+[@@__reduce__]
+let struct_carriers (fields: struct_fields) (field: field_of fields) =
+  (get_field fields field).carrier
 
-to translate t
+[@@__reduce__]
+let struct_pcms (tag: string) (fields: struct_fields) (field: field_of fields)
+: pcm (struct_carriers fields field)
+= (get_field fields field).pcm
 
-  typedef_t: typedef t = { ... }
-
-to translate struct tag { S s; ... }
-
-  assume val struct (tag: string) (fields: list (string * typedef)): Type
-  assume val mk_struct_typedef (tag: string) (fields: list (string * typedef)):
-    typedef (struct tag ["s", typedef_S; ..))
-  
-  typedef_struct_tag: typedef (struct "tag" ["s", typedef_S; ..]) =
-     mk_struct_typedef "tag" ["s", typedef_S; ..]
-
-to translate struct loop { struct loop *again; }
-
-// Done (assuming can store pointers in heap)
-  carrier: Type0; 
-  pcm: pcm carrier; 
-
-view_type = {loop: ref struct_loop_carrier struct_loop_pcm}
-
-mk_view_type
-  (carrier: Type0)
-  (pcm: pcm carrier)
--> view_type : {loop: ref struct_loop_carrier struct_loop_pcm}
-
-mk_rec_typedef:
-  (carrier: Type0)
-  (pcm: pcm carrier)
--> t:typedef (mk_view_type carrier pcm) { t.carrier == carrier /\ t.pcm == pcm}
-
-noeq type typedef = { 
-
-// _
-  view_type: Type0; 
-
-// Should be fine
-  can_view_unit: bool; 
-  view: sel_view pcm view_type can_view_unit; 
-} 
-
-  typedef_struct_loop_f (recur:typedef)
-  : typedef (struct "loop" ["again", ref_typedef recur.carrier recur.pcm])
-  = mk_struct_typedef "loop" ["again", ref_typedef recur.carrier recur.pcm]
-
-  typedef_struct_loop
-  : typedef (struct "loop"
-      ["again",
-       ref_typedef
-         typedef_struct_loop.carrier
-         typedef_struct_loop.pcm])
-  = typedef_struct_loop_f typedef_struct_loop
-
-*)
-
-/// TODO Would be nice to have somtehing like this but proofs get tricky
-
-/// struct_put and struct_get are sound w.r.t. a model of structs as n-tuples
-
-(* BEGIN public *)
-
-let rec list_fn_args (dom: list Type) = match dom with
-  | [] -> unit
-  | d :: dom -> d & list_fn_args dom
-
-let rec list_apply #dom #b (f: dom `list_fn` b) (xs: list_fn_args dom): b = match dom with
-  | [] -> f
-  | a :: dom ->
-    let (x, xs): a & list_fn_args dom = xs in
-    let f: a -> dom `list_fn` b = f in
-    f x `list_apply` xs
-
-let rec struct_get_model
-  (#tag: string) (#fields: struct_fields) 
-  (vs: list_fn_args (mk_struct_ty_dom tag fields))
-  (field: field_of fields)
-: (get_field fields field).view_type
-= match fields with
-  | [] -> assert false
-  | (field', td) :: fields ->
-    let (v, vs): td.view_type & list_fn_args (mk_struct_ty_dom tag fields) = vs in
-    if field = field' then v else struct_get_model vs field
-
-let rec struct_put_model
-  (#tag: string) (#fields: struct_fields) 
-  (vs: list_fn_args (mk_struct_ty_dom tag fields))
-  (field: field_of fields)
-  (v: (get_field fields field).view_type)
-: list_fn_args (mk_struct_ty_dom tag fields)
-= match fields with
-  | [] -> vs
-  | (field', td) :: fields ->
-    let (v', vs): td.view_type & list_fn_args (mk_struct_ty_dom tag fields) = vs in
-    if field = field' then (v, vs) else (v', struct_put_model vs field v)
-
-(* END public *)
-
-val struct_get_sound
-  (#tag: string) (#fields: struct_fields) 
-  (vs: list_fn_args (mk_struct_ty_dom tag fields))
-  (field: field_of fields)
-: Lemma (
-    (mk_struct tag fields `list_apply` vs) `struct_get` field ==
-    struct_get_model vs field)
-
-(*
-let rec struct_get_sound #tag #fields vs field : Lemma (ensures
-    (mk_struct tag fields `list_apply` vs) `struct_get` field ==
-    struct_get_model vs field) (decreases fields) = match fields with
-  | [] -> ()
-  | (field', td) :: fields ->
-    let (v, vs): td.view_type & list_fn_args (mk_struct_ty_dom tag fields) = vs in
-    let field: field_of ((field', td) :: fields) = field in
-    if field = field' then begin
-      let f = mk_struct tag ((field', td) :: fields) in
-      assert ((list_apply #(mk_struct_ty_dom tag ((field', td) :: fields)) f (v, vs)) `struct_get` field ==
-        begin
-          let (x, xs): (struct_field_view_type (field', td) & list_fn_args (mk_struct_ty_dom tag fields)) = (v, vs) in
-          let f: struct_field_view_type (field', td) -> (mk_struct_ty_dom tag fields `list_fn` struct tag fields) = admit() in
-          f x `list_apply` xs
-        end);
-      assume ((list_apply #(mk_struct_ty_dom tag ((field', td) :: fields)) (mk_struct tag ((field', td) :: fields)) (v, vs)) `struct_get` field == v)
-    end else admit()//struct_get_sound #tag #fields vs field
-    *)
+val struct_pcm_carrier (tag: string) (fields: struct_fields): Type0
+val struct_pcm (tag: string) (fields: struct_fields): pcm (struct_pcm_carrier tag fields)
+(*** END PUBLIC *)
 
 let struct_pcm_carrier tag fields = restricted_t (field_of fields) (struct_carriers fields)
 
 let struct_pcm tag fields = prod_pcm (struct_pcms tag fields)
+
+(**** BEGIN PUBLIC *)
+let struct_field_carrier ((_, td): string * typedef): Type = td.carrier
+
+let mk_struct_pcm_ty_dom (tag: string) (fields: list (string * typedef)): list Type =
+  map struct_field_carrier fields
+
+let mk_struct_pcm_ty (tag: string) (fields: struct_fields): Type =
+  mk_struct_pcm_ty_dom tag fields `list_fn` struct_pcm_carrier tag fields
+
+/// A struct PCM carrier literal
+val mk_struct_pcm (tag: string) (fields: struct_fields): mk_struct_pcm_ty tag fields
+(**** END PUBLIC *)
 
 let rec mk_struct_pcm (tag: string) (fields: struct_fields)
 : mk_struct_pcm_ty tag fields
@@ -200,6 +239,78 @@ let rec mk_struct_pcm (tag: string) (fields: struct_fields)
       in on_dom _ h
     in
     list_fn_map lift_struct f
+
+(**** BEGIN PUBLIC *)
+
+/// Reading a pcm_struct_carrier field
+val struct_pcm_get
+  (#tag: string) (#fields: struct_fields)
+  (x: struct_pcm_carrier tag fields) (field: field_of fields)
+: (get_field fields field).carrier
+
+/// Writing a struct_pcm_carrier field
+val struct_pcm_put
+  (#tag: string) (#fields: struct_fields)
+  (x: struct_pcm_carrier tag fields)
+  (field: field_of fields)
+  (v: (get_field fields field).carrier)
+: struct_pcm_carrier tag fields
+
+/// For a fixed field name, struct_pcm_get and struct_pcm_put form a lens
+
+val struct_pcm_get_put 
+  (#tag: string) (#fields: struct_fields)
+  (x: struct_pcm_carrier tag fields)
+  (field: field_of fields)
+  (v: (get_field fields field).carrier)
+: Lemma (struct_pcm_put x field v `struct_pcm_get` field == v)
+  [SMTPat (struct_pcm_put x field v `struct_pcm_get` field)]
+
+val struct_pcm_put_get
+  (#tag: string) (#fields: struct_fields)
+  (x: struct_pcm_carrier tag fields)
+  (field: field_of fields)
+: Lemma (struct_pcm_put x field (x `struct_pcm_get` field) == x)
+  [SMTPat (struct_pcm_put x field (x `struct_pcm_get` field))]
+
+val struct_pcm_put_put
+  (#tag: string) (#fields: struct_fields)
+  (x: struct_pcm_carrier tag fields)
+  (field: field_of fields)
+  (v w: (get_field fields field).carrier)
+: Lemma (struct_pcm_put (struct_pcm_put x field v) field w == struct_pcm_put x field w)
+  [SMTPat (struct_pcm_put (struct_pcm_put x field v) field w)]
+
+/// struct_pcm_get/struct_pcm_put pairs for different fields don't interfere with each other
+
+val struct_pcm_get_put_ne
+  (#tag: string) (#fields: struct_fields)
+  (x: struct_pcm_carrier tag fields)
+  (field1: field_of fields)
+  (field2: field_of fields)
+  (v: (get_field fields field1).carrier)
+: Lemma
+    (requires field1 =!= field2)
+    (ensures struct_pcm_put x field1 v `struct_pcm_get` field2 == x `struct_pcm_get` field2)
+  [SMTPat (struct_pcm_put x field1 v `struct_pcm_get` field2)]
+  
+val struct_pcm_put_put_ne
+  (#tag: string) (#fields: struct_fields)
+  (x: struct_pcm_carrier tag fields)
+  (field1: field_of fields)
+  (v: (get_field fields field1).carrier)
+  (field2: field_of fields)
+  (w: (get_field fields field2).carrier)
+: Lemma
+    (requires field1 =!= field2)
+    (ensures
+      struct_pcm_put (struct_pcm_put x field1 v) field2 w ==
+      struct_pcm_put (struct_pcm_put x field2 w) field1 v)
+
+/// View a struct_pcm_carrier as a struct
+val struct_view (tag: string) (fields: struct_fields)
+: sel_view (struct_pcm tag fields) (struct tag fields) false
+(**** END PUBLIC *)
 
 let struct_pcm_get x field = x field
 
@@ -219,7 +330,58 @@ let struct_pcm_put_put_ne x field1 v field2 w =
    assert (
      struct_pcm_put (struct_pcm_put x field1 v) field2 w `feq`
      struct_pcm_put (struct_pcm_put x field2 w) field1 v)
+     
+(**** BEGIN PUBLIC *)
+// /// View a struct_pcm_carrier as a struct
+// val struct_view (tag: string) (fields: struct_fields) (fields': struct_fields{normalize_term (fields' \subset fields) == true})
+// : sel_view (struct_pcm tag fields) (struct tag fields') false
+// 
+// val struct_view (tag: string) (fields: struct_fields) (fields': struct_fields)
+// : sel_view (struct_pcm tag fields) (struct tag (normalize (fields - fields'))) false
+// 
+// struct_view_convert #opened
+//   (v: struct_view tag fields fields'1)
+// : SteelGhost (struct_view tag fields fields'2) opened
+//     (p `pts_to_view` v)
+//     (fun w -> (p `pts_to_view` w))
+//     (requires fun _ -> normalize (fields - fields'1 == fields - fields'2))
+//     (ensures fun h w h' -> forall field. field in (fields - fields'1) ==>
+//        h (p `pts_to_view` v) `struct_get` field == 
+//        h' (p `pts_to_view` w) `struct_get` field)
+// 
+// struct_view_convert
+//   (v: struct_view tag fields fields'1)
+// : Pure (struct_view tag fields fields'2)
+//     (requires normalize (fields - fields'1 == fields - fields'2))
+//     (ensures fun w -> True)
+//
+// val struct_view (tag: string) (fields: struct_fields) (fields': struct_fields) (fields_fields': struct_fields) (heq: squash (fields_fields' == normalize_term (fields - fields')))
+// : sel_view (struct_pcm tag fields) (struct tag fields_fields') false
 
+// struct_view tag fields fields' (_ by (T.norm _; T.trefl ()))
+
+/// Typedef for struct from typedefs for its fields
+(*
+let typedef_struct (tag: string) (fields: struct_fields): typedef = {
+  carrier = struct_pcm_carrier tag fields; 
+  pcm = struct_pcm tag fields;
+  view_type = struct tag fields;
+  view = struct_view tag fields;
+}
+*)
+
+/// Connections for fields of structs
+
+(*
+val struct_field
+  (tag: string) (fields: struct_fields) (field: field_of fields)
+: connection (struct_pcm tag fields) (struct_pcms tag fields field)
+*)
+
+/// Explode and recombine
+(**** END PUBLIC *)
+
+(*
 let field_views (tag: string) (fields: struct_fields) (field: field_of fields)
 : sel_view (struct_pcms tag fields field) (struct_view_types fields field) false
 = (get_field fields field).view
@@ -284,6 +446,7 @@ let struct_view tag fields = {
 }
 
 let struct_field tag fields field = struct_field (struct_pcms tag fields) field
+*)
 
 /// TODO move and dedup with Steel.C.Ptr.fst
 
